Px86 ptoa: finish proof w/o admit
Signed-off-by: Kyeongmin Cho <kyeongmin.cho@kaist.ac.kr>

src/axiomatic/TsoSimLocal.v
@@ -493,3 +493,72 @@ Proof.
            end;
       eauto 10 using union_l, union_r.
 Qed.
+
+Definition sim_local_lper_end ex loc :=
+  (⦗ex.(Execution.label_is) (Label.is_flushopting loc)⦘ ⨾
+   Execution.po).
+
+Lemma sim_local_lper_end_step ex loc:
+  sim_local_lper_end ex loc =
+  (sim_local_lper_end ex loc ∪
+   (⦗ex.(Execution.label_is) (Label.is_flushopting loc)⦘)) ⨾
+  Execution.po_adj.
+Proof.
+  unfold sim_local_lper_end.
+  rewrite ? (union_seq' Execution.po_adj), ? seq_assoc, ? union_assoc.
+  rewrite Execution.po_po_adj at 1.
+  rewrite (clos_refl_union Execution.po).
+  replace ((Execution.po ∪ eq) ⨾ Execution.po_adj)
+    with (Execution.po ⨾ Execution.po_adj ∪ eq ⨾ Execution.po_adj); cycle 1.
+  { rewrite union_seq. ss. }
+  rewrite eq_seq.
+  rewrite ? (seq_union' (Execution.po ⨾ Execution.po_adj) Execution.po_adj), ? seq_assoc, ? union_assoc.
+  funext. i. funext. i. propext. econs; i.
+  - repeat match goal with
+           | [H: (_ ∪ _) _ _ |- _] => inv H
+           end;
+      eauto 10 using union_l, union_r.
+  - repeat match goal with
+           | [H: (_ ∪ _) _ _ |- _] => inv H
+           end;
+      eauto 10 using union_l, union_r.
+Qed.
+
+Definition sim_local_per_end ex loc :=
+  (⦗ex.(Execution.label_is) (Label.is_flushing loc)⦘ ⨾
+   Execution.po) ∪
+
+  (⦗ex.(Execution.label_is) (Label.is_flushopting loc)⦘ ⨾
+   Execution.po ⨾
+   ⦗ex.(Execution.label_is) (Label.is_persist_barrier)⦘ ⨾
+   Execution.po).
+
+Lemma sim_local_per_end_step ex loc:
+  sim_local_per_end ex loc =
+  (sim_local_per_end ex loc ∪
+   ((⦗ex.(Execution.label_is) (Label.is_flushing loc)⦘) ∪
+
+    (⦗ex.(Execution.label_is) (Label.is_flushopting loc)⦘ ⨾
+     Execution.po ⨾
+     ⦗ex.(Execution.label_is) (Label.is_persist_barrier)⦘))) ⨾
+  Execution.po_adj.
+Proof.
+  unfold sim_local_per_end.
+  rewrite ? (union_seq' Execution.po_adj), ? seq_assoc, ? union_assoc.
+  rewrite Execution.po_po_adj at 1 3.
+  rewrite (clos_refl_union Execution.po).
+  replace ((Execution.po ∪ eq) ⨾ Execution.po_adj)
+    with (Execution.po ⨾ Execution.po_adj ∪ eq ⨾ Execution.po_adj); cycle 1.
+  { rewrite union_seq. ss. }
+  rewrite eq_seq.
+  rewrite ? (seq_union' (Execution.po ⨾ Execution.po_adj) Execution.po_adj), ? seq_assoc, ? union_assoc.
+  funext. i. funext. i. propext. econs; i.
+  - repeat match goal with
+           | [H: (_ ∪ _) _ _ |- _] => inv H
+           end;
+      eauto 10 using union_l, union_r.
+  - repeat match goal with
+           | [H: (_ ∪ _) _ _ |- _] => inv H
+           end;
+      eauto 10 using union_l, union_r.
+Qed.
