src/equiv/TsoPFtoA4SL.v
@@ -273,13 +273,21 @@ Proof.
       all: try by rewrite List.app_length; s; lia.
       all: try rewrite List.nth_error_app2, Nat.sub_diag; ss.
       all: destruct l; ss.
-    + i. rewrite sim_local_per_step. rewrite inverse_step.
-      rewrite inverse_union. ii. des; [apply PER|]; eauto.
+    + i. rewrite sim_local_lper_end_step. rewrite inverse_step.
+      rewrite inverse_union. ii. des; [apply LPER_END|]; eauto.
+      inv EID. obtac.
+      exploit EX2.(LABELS); eauto; ss.
+      { rewrite List.app_length; s; lia. }
+      rewrite List.nth_error_app2, Nat.sub_diag; ss.
+      destruct l; ss.
+    + i. rewrite sim_local_per_end_step. rewrite inverse_step.
+      rewrite inverse_union. ii. des; [apply PER_END|]; eauto.
       inv EID. obtac.
       all: exploit EX2.(LABELS); eauto; ss.
       all: try by rewrite List.app_length; s; lia.
       all: try rewrite List.nth_error_app2, Nat.sub_diag; ss.
-      all: destruct l; ss.
+      * destruct l; ss.
+      * destruct l0; ss.
   - (* write *)
     exploit sim_trace_sim_th; try exact TRACE; eauto. intro TH_tmp.
     exploit lastn_sub_S1; try exact EU; eauto. intro TRT. des.
@@ -389,13 +397,21 @@ Proof.
       all: try by rewrite List.app_length; s; lia.
       all: try rewrite List.nth_error_app2, Nat.sub_diag; ss.
       all: destruct l; ss.
-    + i. rewrite sim_local_per_step. rewrite inverse_step.
-      rewrite inverse_union. ii. des; [apply PER|]; eauto.
+    + i. rewrite sim_local_lper_end_step. rewrite inverse_step.
+      rewrite inverse_union. ii. des; [apply LPER_END|]; eauto.
+      inv EID. obtac.
+      exploit EX2.(LABELS); eauto; ss.
+      { rewrite List.app_length; s; lia. }
+      rewrite List.nth_error_app2, Nat.sub_diag; ss.
+      destruct l; ss.
+    + i. rewrite sim_local_per_end_step. rewrite inverse_step.
+      rewrite inverse_union. ii. des; [apply PER_END|]; eauto.
       inv EID. obtac.
       all: exploit EX2.(LABELS); eauto; ss.
       all: try by rewrite List.app_length; s; lia.
       all: try rewrite List.nth_error_app2, Nat.sub_diag; ss.
-      all: destruct l; ss.
+      * destruct l; ss.
+      * destruct l0; ss.
   - (* rmw *)
     exploit sim_trace_sim_th; try exact TRACE; eauto. intro TH_tmp.
     exploit lastn_sub_S1; try exact EU; eauto. intro TRT. des.
@@ -549,18 +565,23 @@ Proof.
       all: try by rewrite List.app_length; s; lia.
       all: try rewrite List.nth_error_app2, Nat.sub_diag; ss.
       all: destruct l; ss.
-    + i. rewrite sim_local_per_step. rewrite inverse_step.
+    + i. rewrite sim_local_lper_end_step. rewrite inverse_step.
+      rewrite inverse_union. ii. des; [apply LPER_END|]; eauto.
+      inv EID. obtac.
+      exploit EX2.(LABELS); eauto; ss.
+      { rewrite List.app_length; s; lia. }
+      rewrite List.nth_error_app2, Nat.sub_diag; ss.
+      destruct l; ss.
+    + i. rewrite sim_local_per_end_step. rewrite inverse_step.
       rewrite ? inverse_union. ii. des.
-      * exploit PER; eauto. i. rewrite <- join_l. ss.
+      * exploit PER_END; eauto. i. rewrite <- join_l. ss.
       * inv EID. inv REL. obtac.
         exploit EX2.(LABELS); eauto; ss.
         { rewrite List.app_length. s. lia. }
         rewrite List.nth_error_app2, Nat.sub_diag; ss. i. inv x0. inv LABEL.
       * inv EID. inv REL. obtac.
-        exploit EX2.(LABELS); eauto; ss.
-        { rewrite List.app_length. s. lia. }
-        rewrite List.nth_error_app2, Nat.sub_diag; ss. i. inv x0.
-        rewrite <- join_r. apply L. econs; eauto.
+        rewrite <- join_r. inv L. inv LC. ss. apply LPER_END0.
+        econs; eauto. econs. simtac.
   - (* rmw_failure *)
     exploit sim_trace_sim_th; try exact TRACE; eauto. intro TH_tmp.
     exploit lastn_sub_S1; try exact EU; eauto. intro TRT. des.
@@ -737,13 +758,21 @@ Proof.
       all: try by rewrite List.app_length; s; lia.
       all: try rewrite List.nth_error_app2, Nat.sub_diag; ss.
       all: destruct l; ss.
-    + i. rewrite sim_local_per_step. rewrite inverse_step.
-      rewrite inverse_union. ii. des; [apply PER|]; eauto.
+    + i. rewrite sim_local_lper_end_step. rewrite inverse_step.
+      rewrite inverse_union. ii. des; [apply LPER_END|]; eauto.
+      inv EID. obtac.
+      exploit EX2.(LABELS); eauto; ss.
+      { rewrite List.app_length; s; lia. }
+      rewrite List.nth_error_app2, Nat.sub_diag; ss.
+      destruct l; ss.
+    + i. rewrite sim_local_per_end_step. rewrite inverse_step.
+      rewrite inverse_union. ii. des; [apply PER_END|]; eauto.
       inv EID. obtac.
       all: exploit EX2.(LABELS); eauto; ss.
       all: try by rewrite List.app_length; s; lia.
       all: try rewrite List.nth_error_app2, Nat.sub_diag; ss.
-      all: destruct l; ss.
+      * destruct l; ss.
+      * destruct l0; ss.
   - (* mfence *)
     inv STEP0. inv ASTATE_STEP; inv ALOCAL_STEP; ss; inv EVENT; ss. splits.
     econs; ss.
@@ -830,18 +859,24 @@ Proof.
       all: try rewrite List.nth_error_app2, Nat.sub_diag; ss.
       all: destruct l; ss.
     + rewrite List.app_length, Nat.add_1_r.
-      i. rewrite sim_local_per_step. rewrite inverse_step.
+      i. rewrite sim_local_lper_end_step. rewrite inverse_step.
+      rewrite inverse_union. ii. des; [apply LPER_END|]; eauto.
+      inv EID. obtac.
+      exploit EX2.(LABELS); eauto; ss.
+      { rewrite List.app_length; s; lia. }
+      rewrite List.nth_error_app2, Nat.sub_diag; ss.
+      destruct l; ss.
+    + rewrite List.app_length, Nat.add_1_r.
+      i. rewrite sim_local_per_end_step. rewrite inverse_step.
       rewrite ? inverse_union. ii. des.
-      * exploit PER; eauto. i. rewrite <- join_l. ss.
+      * exploit PER_END; eauto. i. rewrite <- join_l. ss.
       * inv EID. inv REL. obtac.
         exploit EX2.(LABELS); eauto; ss.
         { rewrite List.app_length. s. lia. }
         rewrite List.nth_error_app2, Nat.sub_diag; ss. i. inv x0. inv LABEL.
       * inv EID. inv REL. obtac.
-        exploit EX2.(LABELS); eauto; ss.
-        { rewrite List.app_length. s. lia. }
-        rewrite List.nth_error_app2, Nat.sub_diag; ss. i. inv x0.
-        rewrite <- join_r. apply L. econs; eauto.
+        rewrite <- join_r. inv L. inv LC. ss. apply LPER_END0.
+        econs; eauto. econs. simtac.
   - (* sfence *)
     inv STEP0. inv ASTATE_STEP; inv ALOCAL_STEP; ss; inv EVENT; ss. splits.
     econs; ss.
@@ -918,18 +953,24 @@ Proof.
       all: try rewrite List.nth_error_app2, Nat.sub_diag; ss.
       all: destruct l; ss.
     + rewrite List.app_length, Nat.add_1_r.
-      i. rewrite sim_local_per_step. rewrite inverse_step.
+      i. rewrite sim_local_lper_end_step. rewrite inverse_step.
+      rewrite inverse_union. ii. des; [apply LPER_END|]; eauto.
+      inv EID. obtac.
+      exploit EX2.(LABELS); eauto; ss.
+      { rewrite List.app_length; s; lia. }
+      rewrite List.nth_error_app2, Nat.sub_diag; ss.
+      destruct l; ss.
+    + rewrite List.app_length, Nat.add_1_r.
+      i. rewrite sim_local_per_end_step. rewrite inverse_step.
       rewrite ? inverse_union. ii. des.
-      * exploit PER; eauto. i. rewrite <- join_l. ss.
+      * exploit PER_END; eauto. i. rewrite <- join_l. ss.
       * inv EID. inv REL. obtac.
         exploit EX2.(LABELS); eauto; ss.
         { rewrite List.app_length. s. lia. }
         rewrite List.nth_error_app2, Nat.sub_diag; ss. i. inv x0. inv LABEL.
       * inv EID. inv REL. obtac.
-        exploit EX2.(LABELS); eauto; ss.
-        { rewrite List.app_length. s. lia. }
-        rewrite List.nth_error_app2, Nat.sub_diag; ss. i. inv x0.
-        rewrite <- join_r. apply L. econs; eauto.
+        rewrite <- join_r. inv L. inv LC. ss. apply LPER_END0.
+        econs; eauto. econs. simtac.
   - (* dowhile *)
     inv ASTATE_STEP; inv ALOCAL_STEP; ss; inv EVENT; ss. splits.
     + econs; ss; try by apply L.
@@ -1005,13 +1046,29 @@ Proof.
       inversion e. subst. inv H0.
       * rewrite <- join_r, <- join_l. apply L. econs; eauto.
       * repeat rewrite <- join_r. apply L. econs; eauto.
-    + i. rewrite sim_local_per_step. rewrite inverse_step.
-      rewrite inverse_union. ii. des; [apply PER|]; eauto.
+    + i. rewrite sim_local_lper_end_step. rewrite inverse_step.
+      rewrite inverse_union. ii. des.
+      * inv EID. inv REL. obtac. funtac; cycle 1.
+        { inv L. inv LC. ss. apply LPER_END0. econs; eauto. econs. simtac. }
+        inversion e. subst. rewrite <- join_l.
+        inv L. inv LC. ss. apply LPER_END0. econs; eauto. econs. simtac.
+      * inv EID. obtac.
+        exploit EX2.(LABELS); eauto; ss.
+        { rewrite List.app_length. s. lia. }
+        rewrite List.nth_error_app2, Nat.sub_diag; ss. i. inv x0.
+        rewrite EX2.(XVEXT); cycle 1.
+        { ss. rewrite List.app_length. ss. unfold ALocal.next_eid. clear. lia. }
+        condtac; cycle 1.
+        { rewrite Nat.eqb_neq in *. ss. }
+        ss. eqvtac. inv VLOC. rewrite VAL. ss.
+    + i. rewrite sim_local_per_end_step. rewrite inverse_step.
+      rewrite inverse_union. ii. des; [apply PER_END|]; eauto.
       inv EID. obtac.
       all: exploit EX2.(LABELS); eauto; ss.
       all: try by rewrite List.app_length; s; lia.
       all: try rewrite List.nth_error_app2, Nat.sub_diag; ss.
-      all: destruct l; ss.
+      * destruct l; ss.
+      * destruct l0; ss.
   - (* flush *)
     inv STEP0. inv ASTATE_STEP; inv ALOCAL_STEP; ss; inv EVENT; ss. splits.
     econs; ss.
@@ -1084,23 +1141,30 @@ Proof.
       rewrite <- join_r.
       inv COHMAX. specialize (COHMAX0 mloc0). rewrite <- COHMAX0.
       apply VWN0. econs; eauto.
-    + i. rewrite sim_local_per_step. rewrite inverse_step.
+    + i. rewrite sim_local_lper_end_step. rewrite inverse_step.
       rewrite inverse_union. ii. des.
-      { exploit PER; eauto. i. funtac. inversion e. subst. rewrite <- join_l. ss. }
+      { exploit LPER_END; eauto. i. funtac. inversion e. subst. rewrite <- join_l. ss. }
+      inv EID. obtac.
+      exploit EX2.(LABELS); eauto; ss.
+      { rewrite List.app_length; s; lia. }
+      rewrite List.nth_error_app2, Nat.sub_diag; ss.
+      destruct l; ss.
+    + i. rewrite sim_local_per_end_step. rewrite inverse_step.
+      rewrite inverse_union. ii. des.
+      { exploit PER_END; eauto. i. funtac. inversion e. subst. rewrite <- join_l. ss. }
       inv EID. inv REL; cycle 1.
-      { inv H. des. inv H1. inv H2.
+      { obtac.
         exploit EX2.(LABELS); eauto; ss.
         { rewrite List.app_length. s. lia. }
-        rewrite List.nth_error_app2, Nat.sub_diag; ss. i. inv x0. ss.
+        rewrite List.nth_error_app2, Nat.sub_diag; ss. i. inv x1. ss.
       }
       obtac.
       exploit EX2.(LABELS); eauto; ss.
       { rewrite List.app_length. s. lia. }
       rewrite List.nth_error_app2, Nat.sub_diag; ss. i. inv x0.
-      funtac; cycle 1.
-      { exfalso. eqvtac. apply c. inv VLOC. ss. }
-      inversion e. subst.
-      rewrite <- join_r.
-      inv COHMAX. specialize (COHMAX0 mloc0). rewrite <- COHMAX0.
-      apply VWN0. econs; eauto.
+      rewrite EX2.(XVEXT); cycle 1.
+      { ss. rewrite List.app_length. ss. unfold ALocal.next_eid. clear. lia. }
+      condtac; cycle 1.
+      { rewrite Nat.eqb_neq in *. ss. }
+      ss. eqvtac. inv VLOC. rewrite VAL. ss.
 Qed.
